compose/SimSymbId.v
@@ -10,8 +10,10 @@ Require Import Skeleton.
 Require Import Integers.
 Require Import ASTC.
 Require Import LinkingC.
-Require Import SimSymb.
 Require Import MapsC.
+
+
+Require Import SimDef SimSymb.
 
 
 Set Implicit Arguments.
@@ -30,21 +32,76 @@ Inductive globalenv_preserved {F V: Type} (ge: Genv.t F V) (j: meminj) (bound: b
 
 Print Genv.match_genvs. (* Genv.genv_symb is very annoying *)
 
+(* Notation " 'all1' p" := (forall x0, p x0) (at level 50, no associativity). *)
+(* Notation "p =1= q" := (fun x0 => eq (p x0) (q x0)) (at level 50, no associativity). *)
+
 Inductive sim_skenv (skenv0 skenv1: SkEnv.t): Prop :=
 | sim_skenv_intro
     (NEXT: skenv0.(Genv.genv_next) = skenv1.(Genv.genv_next))
-    (SYMB: skenv0.(Genv.find_symbol) =1= skenv1.(Genv.find_symbol)) (* <--- gives bad name when "intros": x0 *)
+    (SYMB: all1 (skenv0.(Genv.find_symbol) =1= skenv1.(Genv.find_symbol))) (* <--- gives bad name when "intros": x0 *)
     (* (SYMB: forall id, skenv0.(Genv.find_symbol) id = skenv1.(Genv.find_symbol) id) *)
     (DEFS: True) (* TODO: There are almost no info except unit. Also, flesh will overwrite these info. *)
+.
+
+Inductive closed (u: unit) (sk_src sk_tgt: Sk.t): Prop :=
+| closed_intro
+    (SIM: match_program (fun _ => sim_fun) eq sk_src sk_tgt)
 .
 
 Global Program Instance SimSymbId: SimSymb.class := {
   t := unit;
   coverage := bot2;
   kept := bot2;
+  closed := closed;
   sim_skenv (_: unit) := sim_skenv;
 }
 .
+Next Obligation.
+  esplits; eauto. ss.
+Qed.
+Next Obligation.
+  econs; ss; eauto.
+  ii; ss.
+  inv CLOSED.
+  unfold match_program in *.
+  generalize (Genv.globalenvs_match SIM); intro SIMGE.
+  inv SIMGE.
+  admit "this should hold.".
+Qed.
+Next Obligation.
+  exists tt.
+  split.
+  - ss.
+  - econs; eauto. inv CLOSED0. inv CLOSED1.
+  admit "This should hold".
+  Print TransfLink.
+  (* exploit link_match_program; eauto. *)
+Qed.
+(* Next Obligation. *)
+(*   inv CLOSED. clear_tac. *)
+(*   assert(SIMID: forall id, (prog_defmap sk_src) ! id = (prog_defmap sk_tgt) ! id). *)
+(*   { i. eapply NOCOVER; eauto. } clear NOCOVER. *)
+(*   u. ss. *)
+(*   econs; eauto. *)
+(*   - admit "this should hold, if not, 1) add uniqueness condition on good_prog to make it hold. *)
+(* 2) Replace Genv.globalenv with my_globalenv, which makes it unique". *)
+(*   - intro id. *)
+(*     specialize (SIMID id). *)
+(*     generalize Genv.find_def_symbol. intro LEMMA. *)
+(*     destruct ((prog_defmap sk_src) ! id) eqn:T. *)
+(*     + eapply LEMMA in T. symmetry in SIMID. eapply LEMMA in SIMID. des. *)
+(*       rewrite T. rewrite SIMID. ss. *)
+(*     + *)
+(*     admit "this should hold, if not, add uniqueness condition on good_prog to make it hold.". *)
+(*     ss. *)
+(* Qed. *)
+Next Obligation.
+  inv CLOSED.
+  unfold match_program in *.
+  generalize (Genv.globalenvs_match SIM); intro SIMGE.
+  inv SIMGE.
+  econs; eauto.
+Qed.
 Next Obligation.
   inv LESRC.
   inv LETGT.
