proof/Ord.v
@@ -3,7 +3,7 @@ Require Import CoqlibC.
 Set Implicit Arguments.
 
 
-
+(* Naming: Do not use order; 1) "ord" is shorter. 2) "orer_link" will be confusing with "link_order" *)
 Section LINK_WFO.
 
   Variable (idx0 idx1: Type) (ord0: idx0 -> idx0 -> Prop) (ord1: idx1 -> idx1 -> Prop).
@@ -18,34 +18,39 @@ Section LINK_WFO.
           <<ORDB: ordB (f a0) (f a1)>>)
   .
 
-  Let idx := (idx0 + idx1)%type.
+  Definition idx_link := (idx0 + idx1)%type.
 
-  Inductive ord: idx -> idx -> Prop :=
-  | ord_introl
+  Inductive ord_link: idx_link -> idx_link -> Prop :=
+  | ord_link_introl
       idx0a idx0b
       (ORD0: ord0 idx0a idx0b)
     :
-      ord (inl idx0a) (inl idx0b)
-  | ord_intror
+      ord_link (inl idx0a) (inl idx0b)
+  | ord_link_intror
       idx1a idx1b
       (ORD1: ord1 idx1a idx1b)
     :
-      ord (inr idx1a) (inr idx1b)
+      ord_link (inr idx1a) (inr idx1b)
   .
 
-  Theorem link_wfo
+  Theorem ord_link_embedded
+    :
+      <<EMBED0: embedded ord0 (ord_link)>> /\ <<EMBED1: embedded ord1 (ord_link)>>
+  .
+  Proof.
+    esplits; eauto.
+    - eapply embedded_intro with (f := inl). econs; eauto.
+    - eapply embedded_intro with (f := inr). econs; eauto.
+  Qed.
+
+  Theorem ord_link_wf
           
           (WF0: well_founded ord0)
           (WF1: well_founded ord1)
     :
-      exists (idx: Type) (ord: idx -> idx -> Prop),
-        <<EMBED0: embedded ord0 ord>> /\ <<EMBED1: embedded ord1 ord>> /\ <<WF: well_founded ord>>
+      <<WF: well_founded ord_link>>
   .
   Proof.
-    exists idx, ord.
-    esplits; eauto.
-    - eapply embedded_intro with (f := inl). econs; eauto.
-    - eapply embedded_intro with (f := inr). econs; eauto.
     - econs; eauto. i. inv H.
       + generalize dependent idx0a. pattern idx0b. eapply well_founded_ind; eauto. clear idx0b. i.
         econs; eauto. i. inv H0.
@@ -55,4 +60,20 @@ Section LINK_WFO.
         eapply H; eauto.
   Qed.
 
+  Theorem ord_link_spec
+          
+          (WF0: well_founded ord0)
+          (WF1: well_founded ord1)
+    :
+      exists (idx: Type) (ord: idx -> idx -> Prop),
+        <<EMBED0: embedded ord0 ord>> /\ <<EMBED1: embedded ord1 ord>> /\ <<WF: well_founded ord>>
+  .
+  Proof.
+    exists idx_link, ord_link.
+    generalize ord_link_embedded; i.
+    hexploit ord_link_wf; eauto. i; des.
+    esplits; eauto.
+  Qed.
+
 End LINK_WFO.
+
