proof/Pair.v
@@ -20,84 +20,6 @@ Set Implicit Arguments.
 
 
 
-Lemma closed_def_bsim
-      `{SimSymb.class}
-      ss sk_src sk_tgt
-      (CLOSED: closed ss sk_src sk_tgt)
-      id gd
-      (DEFTGT: sk_tgt.(prog_defmap) ! id = Some gd)
-  :
-    <<DEFSRC: sk_src.(prog_defmap) ! id = Some gd>>
-.
-Proof.
-  inv CLOSED.
-  destruct (classic (ss.(SimSymb.coverage) id)).
-  - destruct (classic (ss.(SimSymb.kept) id)).
-    + exploit KEPT; eauto. intro EQ. rewrite EQ. ss.
-    + exploit NOKEPT; eauto. i. congruence.
-  - exploit NOCOVER; eauto. i. congruence.
-Qed.
-
-
-
-Module ModPair.
-
-  Record t: Type := mk {
-    src: Mod.t;
-    tgt: Mod.t;
-    SS:> SimSymb.class;
-    ss: SimSymb.t;
-    wf:= closed ss src.(Mod.sk) tgt.(Mod.sk)
-  }
-  .
-
-  Reset t. (* Need to state SS = SS in SimMem... JMEQ THINGS !!!!!!!!!!!!! *)
-
-Section MODPAIR.
-Context `{SS: SimSymb.class}.
-
-  Record t: Type := mk {
-    src: Mod.t;
-    tgt: Mod.t;
-    ss: SimSymb.t;
-  }
-  .
-
-  Inductive wf `{SimSymb.class} (mp: t): Prop :=
-  | wf_intro
-      (CLOSED: closed mp.(ss) mp.(src).(Mod.sk) mp.(tgt).(Mod.sk))
-      (PUB: mp.(src).(Mod.sk).(prog_public) = mp.(tgt).(Mod.sk).(prog_public))
-      (MAIN: mp.(src).(Mod.sk).(prog_main) = mp.(tgt).(Mod.sk).(prog_main))
-  .
-  (* Design: ModPair only has data, properties are stated in sim_modpair *)
-
-  (* Change sim_modsem to be sensitive to si. *)
-  (* Only when initial memory is respecting si, it can guarantee something. *)
-  (* Q: Can we encode it inside SM? *)
-
-End MODPAIR.
-End ModPair.
-
-
-(* Module ModPair. *)
-
-(*   Record t: Type := { *)
-(*     src: Mod.t; *)
-(*     tgt: Mod.t; *)
-(*     si: symbinj; *)
-(*     (* TODO: unify closed & private *) *)
-(*     closed: symbinj_closed si src tgt; *)
-(*     private: symbinj_private si src tgt; *)
-(*     (* TODO: which unary/binary property it expects *) *)
-(*     (* TODO: analysis *) *)
-(*   } *)
-(*   . *)
-
-(*   (* Change sim_modsem to be sensitive to si. *) *)
-(*   (* Only when initial memory is respecting si, it can guarantee something. *) *)
-(*   (* Q: Can we encode it inside SM? *) *)
-
-(* End ModPair. *)
 
 
 
@@ -209,23 +131,4 @@ End ModSemPair.
 
 
 
-
-
-Module GePair.
-Section GEPAIR.
-
-Context `{SS: SimSymb.class} `{SM: SimMem.class}.
-  Record t: Type := mk {
-    skenv_src: SkEnv.t;
-    skenv_tgt: SkEnv.t;
-    ss: SimSymb.t;
-    msps: list ModSemPair.t;
-  }
-  .
-
-  Definition src (gep: t): Ge.t := (Ge.mk gep.(skenv_src) (List.map (ModSemPair.src) gep.(msps))).
-  Definition tgt (gep: t): Ge.t := (Ge.mk gep.(skenv_tgt) (List.map (ModSemPair.tgt) gep.(msps))).
-
-End GEPAIR.
-End GePair.
 
