proof/SimMod.v
@@ -8,13 +8,13 @@ Require Import Smallstep.
 Require Import CoqlibC.
 Require Import Skeleton.
 Require Import ModSem.
-Require Import SimSymb.
 Require Import Integers.
 Require Import ASTC.
 Require Import Maps.
 Require Import LinkingC.
 
-Require Import Syntax Sem Mod Pair ModSem SimMem SimModSem.
+Require Import Syntax Sem Mod ModSem.
+Require Import SimDef SimSymb SimMem SimModSem.
 
 Set Implicit Arguments.
 
@@ -23,33 +23,90 @@ Set Implicit Arguments.
 
 
 
+
+Module ModPair.
+
+  Record t: Type := mk {
+    src: Mod.t;
+    tgt: Mod.t;
+    SS:> SimSymb.class;
+    ss: SimSymb.t;
+    wf:= SimSymb.closed ss src.(Mod.sk) tgt.(Mod.sk)
+  }
+  .
+
+  Reset t. (* Need to state SS = SS in SimMem... JMEQ THINGS !!!!!!!!!!!!! *)
+
+Section MODPAIR.
+Context `{SS: SimSymb.class} `{SM: @SimMem.class SS}.
+
+  Record t: Type := mk {
+    src: Mod.t;
+    tgt: Mod.t;
+    ss: SimSymb.t;
+  }
+  .
+
+  Inductive sim (mp: t): Prop :=
+  | intro_sim
+      (CLOSED: SimSymb.closed mp.(ss) mp.(src).(Mod.sk) mp.(tgt).(Mod.sk))
+      (PUB: mp.(src).(Mod.sk).(prog_public) = mp.(tgt).(Mod.sk).(prog_public))
+      (MAIN: mp.(src).(Mod.sk).(prog_main) = mp.(tgt).(Mod.sk).(prog_main))
+      (SIMMS: forall
+          skenv_src skenv_tgt
+          (SIMSKENV: SimSymb.sim_skenv mp.(ss) skenv_src skenv_tgt)
+        ,
+          exists (idx: Type) (order: idx -> idx -> Prop),
+            <<SIM: sim_modsem order
+                              (mp.(src).(Mod.get_modsem) skenv_src mp.(src).(Mod.data))
+                              (mp.(tgt).(Mod.get_modsem) skenv_tgt mp.(tgt).(Mod.data))
+                              >>)
+            (* <<SIM: sim_modsempair (ModSemPair.mk *)
+            (*                          (mp.(src).(Mod.get_modsem) skenv_src mp.(src).(Mod.data)) *)
+            (*                          (mp.(tgt).(Mod.get_modsem) skenv_tgt mp.(tgt).(Mod.data)) *)
+            (*                          order)>>) *)
+  .
+  (* Design: ModPair only has data, properties are stated in sim *)
+
+  (* Change sim_modsem to be sensitive to si. *)
+  (* Only when initial memory is respecting si, it can guarantee something. *)
+  (* Q: Can we encode it inside SM? *)
+
+End MODPAIR.
+End ModPair.
+
+
+(* Module ModPair. *)
+
+(*   Record t: Type := { *)
+(*     src: Mod.t; *)
+(*     tgt: Mod.t; *)
+(*     si: symbinj; *)
+(*     (* TODO: unify closed & private *) *)
+(*     closed: symbinj_closed si src tgt; *)
+(*     private: symbinj_private si src tgt; *)
+(*     (* TODO: which unary/binary property it expects *) *)
+(*     (* TODO: analysis *) *)
+(*   } *)
+(*   . *)
+
+(*   (* Change sim_modsem to be sensitive to si. *) *)
+(*   (* Only when initial memory is respecting si, it can guarantee something. *) *)
+(*   (* Q: Can we encode it inside SM? *) *)
+
+(* End ModPair. *)
+
+
+
+
 Section SIM.
 
   Context `{SS: SimSymb.class} `{SM: SimMem.class}.
 
-  Inductive sim_modpair (mp: ModPair.t): Prop :=
-  | intro_sim_modpair
-      (WF: ModPair.wf mp)
-      (SIMMSP: forall
-          skenv_src skenv_tgt
-          (SIMSKENV: SimSymb.sim_skenv mp.(ModPair.ss) skenv_src skenv_tgt)
-        ,
-          exists (idx: Type) (order: idx -> idx -> Prop),
-            <<SIM: sim_modsempair (ModSemPair.mk
-                                     (mp.(ModPair.src).(Mod.get_modsem) skenv_src mp.(ModPair.src).(Mod.data))
-                                     (mp.(ModPair.tgt).(Mod.get_modsem) skenv_tgt mp.(ModPair.tgt).(Mod.data))
-                                     order)>>)
-  .
-
-  Inductive sim_progpair (pp: ProgPair.t): Prop :=
-  | intro_sim_modpairs
-      (SIMMP: List.Forall sim_modpair pp)
-  .
-
   Lemma sim_load_mod
         mp0 mp1
-        (SIM0: sim_modpair mp0)
-        (SIM1: sim_modpair mp1)
+        (SIM0: ModPair.sim mp0)
+        (SIM1: ModPair.sim mp1)
         sk_src
         (LINKSRC: link mp0.(ModPair.src).(Mod.sk) mp1.(ModPair.src).(Mod.sk) = Some sk_src)
     :
@@ -62,17 +119,19 @@ Section SIM.
     Local Opaque Linker_prog.
     unfold Sk.t in *.
     exploit (@link_prog_inv (fundef (option signature)) unit); eauto. intro SPEC.
-    inv SIM0. inv SIM1. clear SIMMSP SIMMSP0. inv WF. inv WF0.
+    inv SIM0. inv SIM1. clear SIMMS SIMMS0.
 
     {
       exploit (link_prog_succeeds mp0.(ModPair.tgt).(Mod.sk) mp1.(ModPair.tgt).(Mod.sk)); eauto.
-        inv SPEC. des. congruence.
+      - inv SPEC. des. congruence.
       - intros ? ? ? TGT0 TGT1.
         exploit closed_def_bsim; try apply TGT0; eauto. intro SRC0.
         exploit closed_def_bsim; try apply TGT1; eauto. intro SRC1.
+        des.
         inv SPEC.
         exploit BOTHHIT; eauto. i; des.
         esplits; eauto; try congruence.
+        exploit sim_def_preserves_link; eauto. i ;des. rewrite LINK. ss.
     }
 
     Print link_prog_check.
