compose/SimDef.v
@@ -1,0 +1,96 @@
+Require Import Events.
+Require Import Values.
+Require Import AST.
+Require Import Asmregs.
+Require Import Memory.
+Require Import Globalenvs.
+Require Import Smallstep.
+Require Import CoqlibC.
+Require Import Skeleton.
+Require Import Integers.
+Require Import ASTC.
+Require Import LinkingC.
+Require Import Maps.
+
+
+Set Implicit Arguments.
+
+
+Inductive sim_sig (sg_src sg_tgt: option signature): Prop :=
+| sim_sig_keep
+    sg
+    (SRC: sg_src = Some sg)
+    (TGT: sg_tgt = Some sg)
+| sim_sig_drop
+    (TGT: sg_tgt = None)
+.
+
+Inductive sim_fun: (fundef (option signature)) -> (fundef (option signature)) -> Prop :=
+| sim_fdef_internal
+    sg_src sg_tgt
+    (SIM: sim_sig sg_src sg_tgt)
+  :
+    sim_fun (Internal sg_src) (Internal sg_tgt)
+| sim_fdef_external
+    ef
+  :
+    sim_fun (External ef) (External ef)
+.
+
+(* Inductive sim_var: (globvar unit) -> (globvar unit) -> Prop := *)
+(* | sim_var_intro *)
+(*     gv *)
+(*   : *)
+(*     sim_var gv gv *)
+(* . *)
+
+Inductive sim_def: (globdef (fundef (option signature)) unit) ->
+                    (globdef (fundef (option signature)) unit) -> Prop :=
+| sim_gfun
+    f_src f_tgt
+    (SIM: sim_fun f_src f_tgt)
+  :
+    sim_def (Gfun f_src) (Gfun f_tgt)
+| sim_gvar
+    (* gv_src gv_tgt *)
+    (* (SIM: sim_var gv_src gv_tgt) *)
+    gv
+  :
+    sim_def (Gvar gv) (Gvar gv)
+.
+
+(* TODO: there should be a general function that lifts rel to option rel *)
+Inductive sim_odef: option (globdef (fundef (option signature)) unit) ->
+                    option (globdef (fundef (option signature)) unit) -> Prop :=
+| sim_odef_some
+    def_src def_tgt
+    (SIM: sim_def def_src def_tgt)
+  :
+    sim_odef (Some def_src) (Some def_tgt)
+| sim_odef_none
+  :
+    sim_odef None None
+.
+
+Lemma sim_def_preserves_link
+      (def_src0 def_src1 def_src: globdef (fundef (option signature)) unit)
+      (LINKSRC: link def_src0 def_src1 = Some def_src)
+      def_tgt0 def_tgt1
+      (SIM0: sim_def def_src0 def_tgt0)
+      (SIM1: sim_def def_src1 def_tgt1)
+  :
+    exists def_tgt, <<LINK: link def_tgt0 def_tgt1 = Some def_tgt>> /\ <<SIM: sim_def def_src def_tgt>>
+.
+Proof.
+  Local Transparent Linker_def.
+  Local Transparent Linker_fundef.
+  ss.
+  unfold link_def in *.
+  inv SIM0; inv SIM1; ss; des_ifs_safe.
+  - inv SIM; inv SIM0; ss; des_ifs_safe; esplits; eauto; repeat (econs; eauto).
+  - esplits; eauto. econs; eauto.
+  Local Opaque Linker_def.
+  Local Opaque Linker_fundef.
+Qed.
+
+
