proof/SimGe.v
@@ -1,0 +1,234 @@
+Require Import Events.
+Require Import Values.
+Require Import AST.
+Require Import Asmregs.
+Require Import Memory.
+Require Import Globalenvs.
+Require Import Smallstep.
+Require Import CoqlibC.
+Require Import Skeleton.
+Require Import ModSem.
+Require Import Integers.
+Require Import ASTC.
+Require Import Maps.
+Require Import LinkingC.
+
+Require Import Syntax Sem Mod ModSem.
+Require Import SimSymb SimMem SimModSem SimMod SimProg Ord.
+
+Set Implicit Arguments.
+
+
+
+
+Module GePair.
+Section GEPAIR.
+
+Context `{SS: SimSymb.class} `{SM: @SimMem.class SS}.
+  Record t: Type := mk {
+    skenv_src: SkEnv.t;
+    skenv_tgt: SkEnv.t;
+    ss: SimSymb.t;
+    mss_src: list ModSem.t;
+    mss_tgt: list ModSem.t;
+    (* msps: list ModSemPair.t; *)
+  }
+  .
+
+  Inductive sim (gep: t): Prop :=
+  | intro_sim
+      (SIMSKENV: SimSymb.sim_skenv gep.(ss) gep.(skenv_src) gep.(skenv_tgt))
+      (idx: Type) (order: idx -> idx -> Prop)
+      (SIMMSS: List.Forall2 (sim_modsem order) gep.(mss_src) gep.(mss_tgt))
+  .
+
+  (* Definition src (gep: t): Ge.t := (Ge.mk gep.(skenv_src) (List.map (ModSemPair.src) gep.(msps))). *)
+  (* Definition tgt (gep: t): Ge.t := (Ge.mk gep.(skenv_tgt) (List.map (ModSemPair.tgt) gep.(msps))). *)
+
+End GEPAIR.
+End GePair.
+
+
+Section SIMGE.
+
+  Context `{SS: SimSymb.class} `{SM: @SimMem.class SS}.
+
+  (* Variable pp: ProgPair.t. *)
+  (* Hypothesis SIMPROG: ProgPair.sim pp. *)
+  (* Let p_src := pp.(ProgPair.src). *)
+  (* Let p_tgt := pp.(ProgPair.tgt). *)
+  (* Variable sk_src sk_tgt: Sk.t. *)
+  (* Hypothesis LINKSRC: p_src.(link_sk) = Some sk_src. *)
+  (* Hypothesis LINKTGT: p_tgt.(link_sk) = Some sk_tgt. *)
+  (* Let skenv_src := sk_src.(Sk.load_skenv). *)
+  (* Let skenv_tgt := sk_tgt.(Sk.load_skenv). *)
+  (* Let mss_src := p_src.(load_modsem) skenv_src. *)
+  (* Let mss_tgt := p_tgt.(load_modsem) skenv_tgt. *)
+  (* Let ge_src := (p_src.(load_genv) skenv_src). *)
+  (* (* TODO: I want to use "sem_src.(globalenv)" here, without unfolding it. *) *)
+  (* Let ge_tgt := (p_tgt.(load_genv) skenv_tgt). *)
+
+
+
+  (* TODO: Using "let" breaks tactics like "des" and "generalize dependent", even after "subst"ing it, *)
+  (* but I don't know why... *)
+
+  Theorem sim_progpair_sim_ge
+          pp
+          (SIMPROG: ProgPair.sim pp)
+          p_src p_tgt
+          (PSRC: p_src = pp.(ProgPair.src))
+          (PTGT: p_tgt = pp.(ProgPair.tgt))
+          sk_src sk_tgt
+          (LINKSRC: p_src.(link_sk) = Some sk_src)
+          (LINKTGT: p_tgt.(link_sk) = Some sk_tgt)
+          skenv_src skenv_tgt
+          (SKENVSRC: skenv_src = sk_src.(Sk.load_skenv))
+          (SKENVTGT: skenv_tgt = sk_tgt.(Sk.load_skenv))
+          mss_src mss_tgt
+          (MSSSRC: mss_src = p_src.(load_modsem) skenv_src)
+          (MSSTGT: mss_tgt = p_tgt.(load_modsem) skenv_tgt)
+          
+    :
+      exists ss_link,
+        <<SIM: GePair.sim (GePair.mk skenv_src skenv_tgt ss_link mss_src mss_tgt)>>
+  .
+  Proof.
+    subst. u. ss.
+    assert(exists ss_link, <<LINKSS: pp.(ProgPair.ss_link) = Some ss_link>> /\
+                           <<CLOSED: SimSymb.closed ss_link sk_src sk_tgt>> /\
+                           <<LINKORDER: Forall (fun mp => linkorder mp.(ModPair.ss) ss_link) pp>>).
+    { u.
+      revert_until pp.
+      induction pp; ii; ss.
+      inv SIMPROG.
+      apply link_list_cons_inv in LINKSRC. apply link_list_cons_inv in LINKTGT. des.
+      exploit IHpp; eauto.
+      i; des.
+      rename pp into pp_tl. rename a into pp_hd. rename ss_link into ss_link_tl.
+      exploit SimSymb.link_preserves_closed; revgoals.
+      { i; des. esplits; eauto.
+        - eapply link_list_cons; eauto.
+        - econs; eauto.
+          + exploit link_linkorder; try apply LINKSS; eauto. i; des. ss.
+          + eapply Forall_impl; eauto.
+            i. ss. eapply linkorder_trans; eauto.
+            exploit link_linkorder; try apply LINKSS; eauto. i; des. ss.
+      }
+      all: eauto.
+      apply H1.
+      (* assert(exists ss_link, <<LINK: link pp_hd.(ModPair.ss) ss_link_tl = Some ss_link>>). *)
+      (* { *)
+      (*   eapply SimSymb.link_success; eauto. *)
+      (*   admit "closed -> coverage <1= privs. Privs are disjoint, assuming they are good_prog". *)
+      (* } *)
+      (* des. exploit link_list_cons; eauto. *)
+      (* esplits; eauto. *)
+      (* exploit SimSymb.link_preserves_closed; revgoals. *)
+      (* [..|i; des; esplits; eauto]. *)
+      (* admit "TODO: closed is monotone!!". *)
+    }
+    des. exists ss_link.
+    remember (Genv.globalenv sk_src) as skenv_src.
+    remember (Genv.globalenv sk_tgt) as skenv_tgt.
+    assert(SIMSKENV: SimSymb.sim_skenv ss_link skenv_src skenv_tgt).
+    { eapply SimSymb.load_respects_ss; eauto. }
+    clear Heqskenv_src Heqskenv_tgt. clear LINKSRC LINKTGT LINKSS CLOSED.
+    assert(SIMMS: exists (idx : Type) (order : idx -> idx -> Prop),
+              Forall2 (sim_modsem order) (pp.(ProgPair.src).(load_modsem) skenv_src)
+                                         (pp.(ProgPair.tgt).(load_modsem) skenv_tgt)).
+    { induction pp.
+      - unshelve esplits; eauto. unshelve econs; eauto.
+      - inv SIMPROG. inv LINKORDER.
+        exploit IHpp; eauto. i; des.
+        inv H1.
+        exploit SIMMS; eauto. { eapply SimSymb.sim_skenv_monotone_ss; eauto. } i; des. clear SIMMS.
+        exists (idx_link idx idx0), (ord_link order order0).
+        ss. u.
+        econs; eauto.
+        + u. eapply embedding_preserves_sim; eauto. eapply ord_link_embedded; eauto.
+        + eapply Forall2_impl; try apply H.
+          i. eapply embedding_preserves_sim; eauto. eapply ord_link_embedded; eauto.
+    }
+    des.
+    econs; eauto.
+  Qed.
+
+End SIMGE.
+
+(* Section SIMGE. *)
+
+(*   Context `{SS: SimSymb.class} `{SM: @SimMem.class SS}. *)
+
+(*   (* Hypothesis CLOSED: closed ss_link sk_src sk_tgt. *) *)
+
+(*   Theorem sim_progpair_sim_ge *)
+(*     : *)
+(*       exists ss_link, *)
+(*         <<SIM: GePair.sim (GePair.mk skenv_src skenv_tgt ss_link mss_src mss_tgt)>> *)
+(*   . *)
+(*   Proof. *)
+(*     ss. *)
+(*     subst_locals. u. ss. *)
+(*     assert(exists ss_link, pp.(ProgPair.ss_link) = Some ss_link). *)
+(*     { u. *)
+(*       generalize dependent sk_src. (* TODO: This does not work!! Is this a bug?? *) Undo 1. *)
+(*       revert_until pp. *)
+(*       induction pp; ii; ss. *)
+(*       inv SIMPROG. *)
+(*       apply link_list_cons_inv in LINKSRC. apply link_list_cons_inv in LINKTGT. *)
+(*       des. (* TODO: des does not work!! Is this a bug?? *) *)
+(*       destruct  *)
+(*       exploit IHt; eauto. *)
+(*       - ss. *)
+(*       - ss. *)
+(*     } *)
+(*     assert(SIMSKENV: exists ss, SimSymb.sim_skenv ss sk_src.(Sk.load_skenv) sk_tgt.(Sk.load_skenv)). *)
+(*     induction pp; ii; ss. *)
+(*     - inv WF. inv SIMMPS. unfold init_sk in *. ss. *)
+(*       all ltac:(fun H => apply link_list_cons_inv in H). *)
+(*       des. (* TODO: Why des does not work? *) *)
+(*       destruct LINKSRC, LINKTGT; clear LINKSRC LINKTGT; des. *)
+(*       exploit IHt; eauto. *)
+(*       i; des. *)
+(*       esplits; eauto. *)
+(*       { inv  *)
+(*     assert(SIMSKENV: SimSymb.sim_skenv ss_link ge_src.(Ge.skenv) ge_tgt.(Ge.skenv)). *)
+(*     { exploit SimMem.load_respects_ss; eauto. i; des. ss. } *)
+(*     econs; eauto. *)
+(*     inv SIMPROG. *)
+(*     cbn. *)
+(*     clear - SIMMPS SIMSKENV SSLINK. *)
+(*     unfold ProgPair.ss_link in *. *)
+(*     assert(LINKORDER: forall *)
+(*               ss *)
+(*               (IN: List.In ss (map ModPair.ss pp)) *)
+(*             , *)
+(*               <<LO: linkorder ss ss_link>>). *)
+(*     { i. admit "link_list_linkorder". } *)
+(*     subst skenv_src skenv_tgt ge_src ge_tgt p_src p_tgt. *)
+(*     ginduction pp; ii; ss. *)
+(*     unfold flip. inv SIMMPS. *)
+(*     econs; eauto. *)
+(*     - eapply H1; eauto. *)
+(*       eapply SimSymb.sim_skenv_monotone_ss; eauto. *)
+(*       admit "link_list_linkorder". *)
+(*     - eapply IHt; eauto. *)
+(*       admit "link_list_linkorder". *)
+(*   Qed. *)
+
+
+(*   Variable ss_link: SimSymb.t. *)
+(*   Variable sem_src sem_tgt: semantics. *)
+(*   Hypothesis LOADSRC: sem p_src = Some sem_src. *)
+(*   Hypothesis LOADTGT: sem p_tgt = Some sem_tgt. *)
+(*   Hypothesis SSLINK: pp.(ProgPair.ss_link) = Some ss_link. *)
+
+(*   Variable m_src m_tgt: mem. *)
+(*   Hypothesis LOADMEMSRC: sk_src.(Sk.load_mem) = Some m_src. *)
+(*   Hypothesis LOADMEMTGT: sk_tgt.(Sk.load_mem) = Some m_tgt. *)
+
+(*   Theorem sim_modsem *)
+
+(* End SIMGE. *)
+
