proof/SimMemId.v
@@ -43,17 +43,17 @@ Program Instance MemRelId : SimMem.class SimSymbId :=
 Next Obligation.
   ss.
 Qed.
-Next Obligation.
-  eexists (mkrelation _ _).
-  esplits; ss; eauto.
-  inv WF. ss.
-  clear_tac.
-  assert(NOCOVER0: forall id, <<EQ: sk_src.(prog_defmap) ! id = sk_tgt.(prog_defmap) ! id>>).
-  { i. eapply NOCOVER. eauto. }
-  clear NOCOVER.
-  clear_tac.
-  econs; eauto.
-  - admit "This should hold; Maybe ""Genv.init_mem_match"" and ""Genv.init_mem_genv_next"" might help".
-  - admit "This should hold;".
-Qed.
+(* Next Obligation. *)
+(*   eexists (mkrelation _ _). *)
+(*   esplits; ss; eauto. *)
+(*   inv WF. ss. *)
+(*   clear_tac. *)
+(*   assert(NOCOVER0: forall id, <<EQ: sk_src.(prog_defmap) ! id = sk_tgt.(prog_defmap) ! id>>). *)
+(*   { i. eapply NOCOVER. eauto. } *)
+(*   clear NOCOVER. *)
+(*   clear_tac. *)
+(*   econs; eauto. *)
+(*   - admit "This should hold; Maybe ""Genv.init_mem_match"" and ""Genv.init_mem_genv_next"" might help". *)
+(*   - admit "This should hold;". *)
+(* Qed. *)
 
